Add: fst VM (ML)

VM.fsti
@@ -1,75 +1,15 @@
 module VM
 
 (* imported modules *)
-open FStar.List
-open FStar.Heap
+open Structs
 (* ---------------- *)
 
-(* bytecode instruction *)
-type opcode = 
-  | ADD
+(* Creates a new frame and push it to the frame stack *)
+val makeFrame: vm -> codeObj -> (vm * frameObj)
 
-type bytecode = 
-  | CODE: list opcode -> bytecode
+(* Run Frame and then pop it from call stack when you done *)
+val runFrame: vm -> frameObj -> All.ML (vm * pyObj)
 
-(* object code *)
-type codeObj = {
-  code: bytecode;
-  (*
-  .
-  .
-  . 
-  *)
-}
-
-(* Block object *)
-type blockObj = {
-  (* currently executed opcode (type is int in cpyhton) *)
-  b_type: opcode;
-  (* The number of items on the value stack of the frame *)
-  b_level: nat;
-  (* The index of the instruction after the block *)
-  b_handler: nat
-}
-
-
-(* Frame object *)
-noeq type frameObj = {
-  (* Simulates a stack that handles inputs of different types *)
-  dataStack: heap;
-  (* Simulates a stack of blocks*)
-  blockStack: list blockObj
-  (*
-  .
-  .
-  . 
-  *)
-}
-
-
-(* Function Object *)
-type functionObj = {
-  funCode: bytecode
-  (*
-  .
-  .
-  . 
-  *)
-} 
-
-(* VM (thread) *)
-noeq type vm = {
-  (* Simulates a stack of frames *)
-  callStack: list frameObj;
-  (* Simulates a stack of (function name, functionObj) *)
-  functionsEnv: list (string * functionObj);
-  (* Input to vm *)
-  code: codeObj
-  (*
-  .
-  .
-  . 
-  *)
-}
-
+(* Takes in code object and execute it *)
+val runCode: codeObj -> All.ML pyObj
 
