Exec.fst
@@ -1,0 +1,69 @@
+module Exec
+
+(*
+   Req: length(datastack) >= 1
+*)
+let return_value dataStack = List.hd dataStack
+
+(*
+  Req: (length(consts) > i) && (length(datastack) >= 1)
+*)
+let load_const i consts dataStack =
+  let elem = List.nth consts i in
+  let newDataStack = elem::dataStack in
+  newDataStack
+
+(*
+  Req: (length(varnames) > i) && (length(datastack) >= 1)
+*)
+let load_fast i varnames dataStack =
+  let elem = List.nth varnames i in
+  let newDataStack = elem::dataStack in
+  newDataStack
+
+(*
+  Req: (length(varnames) > i) && (length(datastack) >= 1)
+*)
+let store_fast i varnames dataStack =
+  let elem = List.hd dataStack in
+  let newDataStack = List.tail dataStack in
+  let newVarnames = List.mapi (fun k x -> if k = i then elem else x) varnames in
+  (newVarnames, newDataStack)
+
+(*
+  Req: length(datastack) >= 2
+*)
+let binary_add (dataStack: list pyObj) = 
+  let a = List.hd dataStack in
+  let b = List.nth dataStack 1 in
+  let (_, newDataStack) = List.splitAt 2 dataStack in 
+  match (a, b) with
+  | INT(a'), INT(b') -> INT(a' + b')::newDataStack
+  | STRING(a'), STRING(b') -> STRING(a' ^  b')::newDataStack
+  | _, _ -> All.failwith "Error: binary_Add incompatable types"
+
+(*
+   Req: len(frame.fcode.bytecode) >= 1
+*)
+let rec execBytecode frame =
+  let CODE(bc) = frame.fCode.co_code in
+  match bc with
+  | RETURN_VALUE::l -> return_value frame.dataStack
+  | LOAD_CONST(i)::l ->
+    let newDataStack = load_const i (frame.fCode.co_consts) (frame.dataStack) in
+    execBytecode ({frame with dataStack = newDataStack; fCode = {frame.fCode with co_code = CODE l}})
+    
+  | LOAD_FAST(i)::l ->
+    let newDataStack = load_fast i (frame.fCode.co_varnames) (frame.dataStack) in
+    execBytecode ({frame with dataStack = newDataStack; fCode = {frame.fCode with co_code = CODE l}})   
+    
+  | STORE_FAST(i)::l ->
+    let (newVarnames, newDataStack) = store_fast i (frame.fCode.co_varnames) (frame.dataStack) in
+    let newFCode = {frame.fCode with co_code = CODE l; co_varnames = newVarnames} in
+    execBytecode ({frame with dataStack = newDataStack; fCode = newFCode})
+    
+  | BINARY_ADD::l -> 
+    let newDataStack = binary_add (frame.dataStack) in
+    execBytecode ({frame with dataStack = newDataStack; fCode = {frame.fCode with co_code = CODE l}})
+  | [] -> All.failwith "Error: reached empty bytecode array "
+
