Exec.fsti
@@ -1,0 +1,17 @@
+module Exec
+
+(* imported modules *)
+open Structs
+(* ---------------- *)
+
+val return_value: list pyObj -> All.ML pyObj
+
+val load_const: nat -> list pyObj -> list pyObj -> All.ML (list pyObj)
+
+val load_fast: nat -> list pyObj -> list pyObj -> All.ML (list pyObj)
+
+val store_fast: nat -> list pyObj -> list pyObj -> All.ML (list pyObj * list pyObj)
+
+val binary_add: list pyObj -> All.ML (list pyObj)
+
+val execBytecode: frameObj -> All.ML pyObj
