Structs.fsti
@@ -1,0 +1,81 @@
+module Structs
+
+(* bytecode instruction *)
+type opcode = 
+  | LOAD_CONST: nat -> opcode
+  | LOAD_FAST: nat -> opcode
+  | STORE_FAST: nat -> opcode
+  | BINARY_ADD: opcode
+  | RETURN_VALUE: opcode
+  
+type bytecode = 
+  | CODE: l: list opcode -> bytecode
+
+(* The types of data allowed in datastack*)
+noeq type pyObj =
+  | INT: int -> pyObj
+  | STRING: string -> pyObj
+  | NONE
+  | ERR
+  
+(* object code *)
+noeq type codeObj = {
+  co_code: bytecode;
+  co_consts: list pyObj; // elem at index 0 must be None
+  co_varnames: list pyObj
+  (*
+  .
+  .
+  . 
+  *)
+}
+
+(* Block object *)
+noeq type blockObj = {
+  (* currently executed opcode (type is int in cpyhton) *)
+  b_type: opcode;
+  (* The number of items on the value stack of the frame *)
+  b_level: nat;
+  (* The index of the instruction after the block *)
+  b_handler: nat
+}
+
+(* Frame object *)
+noeq type frameObj = {
+  (* Simulates a stack that handles inputs of different types *)
+  dataStack: list pyObj;
+  (* Simulates a stack of blocks*)
+  blockStack: list blockObj;
+  (* code Object that is gonna run in this frame *)
+  fCode: codeObj
+  (*
+  .
+  .
+  . 
+  *)
+}
+
+(* Function Object *)
+noeq type functionObj = {
+  funCode: bytecode
+  (*
+  .
+  .
+  . 
+  *)
+} 
+
+(* VM (thread) *)
+noeq type vm = {
+  (* Simulates a stack of frames *)
+  callStack: list frameObj;
+  (* Simulates a stack of (function name, functionObj) *)
+  functionsEnv: list (string * functionObj);
+  (* Input to vm *)
+  code: codeObj
+  (*
+  .
+  .
+  . 
+  *)
+}
