VM.fst
@@ -1,0 +1,45 @@
+module VM
+
+(* imported modules *)
+open Exec
+(* ---------------- *)
+
+(* Create a new frame and push it in the frame stack *)
+let makeFrame virM code =
+  let frame: frameObj = {dataStack = []; blockStack = []; fCode = code} in
+  let newVM: vm = {virM with callStack = frame::(virM.callStack)} in
+  (newVM, frame)
+
+
+(*
+   - Runs the code in the frame and update the VM once it's done.
+   Req: frame is the top element in the callstack in virM.
+*)
+let runFrame virM frame =
+  (* Execute *) 
+  let result = execBytecode frame in
+  
+  (* Check if result is ERR *)
+  
+  (* Pop the top frame*)
+  let popVM = {virM with callStack = List.tail (virM.callStack)} in
+  (* Push result to the top of the caller frame (top frame in the call stack) *)
+  let callerFrame = List.hd popVM.callStack in
+  let newCallStack = List.tail popVM.callStack in
+  let newCallerFrame = {callerFrame with dataStack =  result::callerFrame.dataStack} in
+  let newVM: vm = {popVM with callStack = newCallerFrame::newCallStack} in
+  (newVM, result)
+
+
+(* Run code object *)
+let runCode code =
+  (* Init the virtual machine *)
+  let initVM: vm = {
+    callStack = [];
+    functionsEnv = []; 
+    code = code
+  } in
+  (* Create global frame to run the byte code instructions in it *)
+  let  virM, globalFrame = makeFrame initVM code in
+  let  newVM, result = runFrame virM globalFrame in
+  result
